TAPLFormalization/BigStep.lean
@@ -1,11 +1,13 @@
 import TAPLFormalization.AST
 import TAPLFormalization.Semantics
+import TAPLFormalization.SemanticsTheorems
 
 inductive BigStep : Term → Term → Prop where
   | value : IsValue v → BigStep v v
   | ifTrue : IsValue v → BigStep t₁ .trueV → BigStep t₂ v
     → BigStep (.ifThenElse t₁ t₂ t₃) v
-  | ifFalse : IsValue v → BigStep t₁ .falseV → BigStep t₃ v → BigStep (.ifThenElse t₁ t₂ t₃) v
+  | ifFalse : IsValue v → BigStep t₁ .falseV → BigStep t₃ v
+    → BigStep (.ifThenElse t₁ t₂ t₃) v
   | succ : IsNumericValue v → BigStep t₁ v → BigStep (.succ t₁) (.succ v)
   | predZero : BigStep t₁ .zero → BigStep (.pred t₁) .zero
   | predSucc : IsNumericValue v → BigStep t₁ (.succ v) → BigStep (.pred t₁) v
@@ -22,7 +24,55 @@ lemma bigStep_of_smallSteps : IsValue v → t ~>* v → BigStep t v := by
   induction t_sts_v <;> grind [BigStep, smallStep_preserves_bigStep]
 
 lemma smallSteps_of_bigStep : IsValue v → BigStep t v → t ~>* v := by
-  sorry
+  intro v_value t_bigst_v
+  induction t_bigst_v
+  case value => constructor
+  case ifTrue v_value t₁_bst_trueV t₂_bst_v ih_trueV ih_v =>
+    rename_i v t₁ t₂ t₃ _
+    let t₁_sts_trueV := ih_trueV (by constructor)
+    let t₂_sts_v := ih_v v_value
+    let sts₁ : t₁.ifThenElse t₂ t₃ ~>* .ifThenElse .trueV t₂ t₃ := smallSteps_in_context
+      (.ifThenElse · t₂ t₃) SmallStep.If t₁_sts_trueV
+    let sts₂ : t₁.ifThenElse t₂ t₃ ~>* t₂ := SmallSteps.trans'.trans sts₁ .IfTrue
+    exact SmallSteps.trans.trans sts₂ t₂_sts_v
+  case ifFalse v_value t₁_bigst_falseV t₂_bst_v ih_falseV ih_v =>
+    rename_i v t₁ t₂ t₃ _
+    let t₁_sts_falseV := ih_falseV (by constructor)
+    let t₂_sts_v := ih_v v_value
+    let sts₁ : t₁.ifThenElse t₃ t₂ ~>* .ifThenElse .falseV t₃ t₂ := smallSteps_in_context
+      (.ifThenElse · t₃ t₂) SmallStep.If t₁_sts_falseV
+    let sts₂ : t₁.ifThenElse t₃ t₂ ~>* t₂ := SmallSteps.trans'.trans sts₁ .IfFalse
+    exact SmallSteps.trans.trans sts₂ t₂_sts_v
+  case succ v_value t_bst_v ih =>
+    apply smallSteps_in_context .succ SmallStep.Succ
+    apply ih
+    cases v_value
+    rename_i v_nv
+    cases v_nv
+    constructor
+    assumption
+  case predZero t_st_zero ih =>
+    let sts₁ := smallSteps_in_context .pred SmallStep.Pred
+      (ih (by repeat constructor))
+    apply SmallSteps.trans'.trans sts₁
+    constructor
+  case predSucc v_nv t_bst_v_succ ih =>
+    let sts₁ := smallSteps_in_context .pred SmallStep.Pred
+      (ih (by constructor; constructor; assumption))
+    apply SmallSteps.trans'.trans sts₁
+    constructor
+    assumption
+  case isZeroZero t_bst_zero ih =>
+    let sts₁ := smallSteps_in_context .isZero SmallStep.IsZero
+      (ih (by repeat constructor))
+    apply SmallSteps.trans'.trans sts₁
+    constructor
+  case isZeroSucc v_nv t_bst_v_succ ih =>
+    let sts₁ := smallSteps_in_context .isZero SmallStep.IsZero
+      (ih (by constructor; constructor; assumption))
+    apply SmallSteps.trans'.trans sts₁
+    constructor
+    assumption
 
 theorem bigStep_iff_smallSteps : IsValue v → (BigStep t v ↔ t ~>* v) := by
   intro v_value
